pulse/src/checker/Pulse.Syntax.Naming.fst
@@ -53,12 +53,12 @@ let close_open_inverse_comp' (c:comp)
     | C_Tot t ->
       close_open_inverse' t x i
 
-    | C_ST s 
-    | C_STGhost s -> 
+    | C_ST s ->
       close_open_inverse' s.res x i;
       close_open_inverse' s.pre x i;      
       close_open_inverse' s.post x (i + 1)
 
+    | C_STGhost n s
     | C_STAtomic n _ s ->    
       close_open_inverse' n x i;    
       close_open_inverse' s.res x i;
@@ -258,8 +258,8 @@ let open_with_gt_ln_comp (c:comp) (i:int) (t:term) (j:nat)
           (ensures open_comp' c t j == c) =
   match c with
   | C_Tot t1 -> open_with_gt_ln t1 i t j
-  | C_ST s
-  | C_STGhost s -> open_with_gt_ln_st s i t j
+  | C_ST s -> open_with_gt_ln_st s i t j
+  | C_STGhost inames s
   | C_STAtomic inames _ s ->
     open_with_gt_ln inames i t j;
     open_with_gt_ln_st s i t j
@@ -285,9 +285,8 @@ let close_comp_with_non_free_var (c:comp) (x:var) (i:nat)
     (ensures close_comp' c x i == c) =
   match c with
   | C_Tot t1 -> close_with_non_freevar t1 x i
-  | C_ST s 
-  | C_STGhost s ->
-    close_with_non_freevar_st s x i
+  | C_ST s -> close_with_non_freevar_st s x i
+  | C_STGhost inames s
   | C_STAtomic inames _ s ->
     close_with_non_freevar inames x i;
     close_with_non_freevar_st s x i
